Introduce is_update for body of updates_slice_frag

src/program_proof/wal/lib.v
@@ -15,6 +15,10 @@ Proof.
   destruct u; rewrite /blockT; val_ty.
 Qed.
 
+Definition is_update (uv: u64*Slice.t) (q:Qp) (u: update.t): iProp Σ :=
+  ⌜uv.1 = u.(update.addr)⌝ ∗
+  is_block uv.2 q u.(update.b).
+
 Definition updates_slice (bk_s: Slice.t) (bs: list update.t): iProp Σ :=
   ∃ bks, is_slice bk_s (struct.t Update.S) 1 (update_val <$> bks) ∗
    [∗ list] _ ↦ b_upd;upd ∈ bks;bs , let '(update.mk a b) := upd in
@@ -23,9 +27,7 @@ Definition updates_slice (bk_s: Slice.t) (bs: list update.t): iProp Σ :=
 
 Definition updates_slice_frag (bk_s: Slice.t) (q:Qp) (bs: list update.t): iProp Σ :=
   ∃ bks, is_slice_small bk_s (struct.t Update.S) q (update_val <$> bks) ∗
-   [∗ list] _ ↦ b_upd;upd ∈ bks;bs,
-       is_block (snd b_upd) q upd.(update.b) ∗
-       ⌜fst b_upd = upd.(update.addr)⌝.
+   [∗ list] _ ↦ uv;upd ∈ bks;bs, is_update uv q upd.
 
 Theorem updates_slice_frag_acc bk_s bs :
   updates_slice bk_s bs -∗
@@ -38,13 +40,15 @@ Proof.
   iSplitR "Hbks".
   - iExists _; iFrame.
     iApply (big_sepL2_mono with "Hupds").
-    intros ? ? [a b]; auto.
+    intros ? ? [a b] **.
+    by iIntros "[$ %]".
   - iIntros "Hupds".
     iDestruct "Hupds" as (bks') "[Hs Hupds]".
     iSpecialize ("Hbks" with "Hs").
     iExists _; iFrame.
     iApply (big_sepL2_mono with "Hupds").
-    intros ? ? [a b]; auto.
+    intros ? ? [a b] **.
+    by iIntros "[% $]".
 Qed.
 
 Theorem updates_slice_to_frag bk_s bs :
@@ -95,9 +99,8 @@ Qed.
 
 Instance is_blocks_AsFractional bks q v :
   fractional.AsFractional
-    ([∗ list] b_upd;upd ∈ bks;v,
-                                (is_block b_upd.2 q upd.(update.b) ∗ ⌜b_upd.1 = upd.(update.addr)⌝))%I
-    (λ q, [∗ list] b_upd;upd ∈ bks;v, (is_block b_upd.2 q upd.(update.b) ∗ ⌜b_upd.1 = upd.(update.addr)⌝))%I
+    ([∗ list] b_upd;upd ∈ bks;v, is_update b_upd q upd)
+    (λ q, [∗ list] b_upd;upd ∈ bks;v, is_update b_upd q upd)%I
     q.
 Proof.
   constructor; auto.
@@ -153,8 +156,7 @@ Theorem wp_SliceGet_updates stk E bk_s bs (i: u64) q (u: update.t) :
   {{{ updates_slice_frag bk_s q bs ∗ ⌜bs !! int.nat i = Some u⌝ }}}
     SliceGet (struct.t Update.S) (slice_val bk_s) #i @ stk; E
   {{{ uv, RET (update_val uv);
-      ⌜uv.1 = u.(update.addr)⌝ ∗
-      is_block uv.2 q u.(update.b) ∗
+      is_update uv q u ∗
       (is_block uv.2 q u.(update.b) -∗ updates_slice_frag bk_s q bs)
   }}}.
 Proof.
@@ -170,9 +172,9 @@ Proof.
   iApply "HΦ".
   iDestruct (big_sepL2_lookup_acc with "Hbks") as "[Hbi Hbks]"; eauto.
   destruct u as [a b]; simpl.
-  iDestruct "Hbi" as "[Hbi <-]".
-  iSplit; first by auto.
-  iFrame.
+  iDestruct "Hbi" as "[%Heq Hbi]".
+  iSplitL "Hbi".
+  { by iFrame. }
   iIntros "Hbi".
   iSpecialize ("Hbks" with "[$Hbi //]").
   iExists _; iFrame.
@@ -190,7 +192,7 @@ Proof.
   iIntros (Φ) "[Hupds %Hlookup] HΦ".
   iDestruct (updates_slice_frag_acc with "Hupds") as "[Hfrag Hupds]".
   wp_apply (wp_SliceGet_updates with "[$Hfrag]"); eauto.
-  iIntros (uv) "(%&Hb&Hrest)".
+  iIntros (uv) "((%&Hb)&Hrest)".
   iApply "HΦ".
   iSplit; auto.
   iFrame.
@@ -245,7 +247,7 @@ Qed.
 Theorem wp_forSlice_updates (I: u64 -> iProp Σ) stk E s q us (body: val) :
   (∀ (i: u64) (uv: u64 * Slice.t) (u: update.t),
       {{{ I i ∗ ⌜(int.nat i < length us)%nat⌝ ∗
-                is_block uv.2 q u.(update.b) ∗
+                is_update uv q u ∗
                 ⌜us !! int.nat i = Some u⌝ }}}
         body #i (update_val uv) @ stk; E
       {{{ RET #(); I (word.add i (U64 1)) ∗
@@ -262,8 +264,7 @@ Proof.
   iDestruct (big_sepL2_length with "Hbs") as %Hlen_eq.
   wp_apply (wp_forSlice
               (fun i => I i ∗
-                       [∗ list] b_upd;upd ∈ bks;us, is_block b_upd.2 q upd.(update.b)
-                       ∗ ⌜b_upd.1 = upd.(update.addr)⌝)%I with "[] [$I0 $Hs $Hbs]").
+                       [∗ list] b_upd;upd ∈ bks;us, is_update b_upd q upd)%I with "[] [$I0 $Hs $Hbs]").
   {
     clear Φ.
     iIntros (i x).
@@ -272,7 +273,7 @@ Proof.
     rewrite list_lookup_fmap in Hlookup.
     apply fmap_Some_1 in Hlookup as [uv [Hlookup ->]].
     destruct (list_lookup_lt _ us (int.nat i) ltac:(word)) as [u Hlookup'].
-    iDestruct (big_sepL2_lookup_acc with "Hbs") as "[[Hb %] Hbs]"; eauto.
+    iDestruct (big_sepL2_lookup_acc with "Hbs") as "[[% Hb] Hbs]"; eauto.
     wp_apply ("Hwp" with "[$HI $Hb]").
     - iPureIntro.
       split; auto.
